src/test/scala/qrhl/tactic/O2HTacTest.scala
@@ -7,16 +7,57 @@ import qrhl.toplevel.{Toplevel, ToplevelTest}
 
 class O2HTacTest extends FunSuite {
   test("o2h tac") {
-    val tl = Toplevel.makeToplevelWithTheory()
+    val tl = Toplevel.makeToplevelWithTheory(List("Empty"))
     tl.run(
       """
         | ambient var q : nat.
         | ambient var rho : program_state.
         | classical var b : bit.
         | classical var Find : bool.
-        | program p := {}.
+        | classical var count : nat.
+        | ambient var o2h_distr : (string set * (string=>bit) * (string=>bit) * unit) distr.
+        | classical var G : string => bit.
+        | classical var H : string => bit.
+        | classical var z : unit.
+        | classical var S : string set.
+        | quantum var X : string.
+        | quantum var Y : bit.
+        | classical var hit : bit.
         |
-        | lemma abs ( Pr[b=1:p(rho)] - Pr[b=1:p(rho)] ) <= 2 * sqrt( (1+real q) * Pr[Find:p(rho)] ).
+        | program Count(O) := { call O; count <- count + 1; }.
+        | adversary Adv_O2H vars z, b, H, X, Y calls ?.
+        |
+        |
+        | program queryG := { on X,Y apply (Uoracle G); }.
+        | program queryGS := {
+        |   hit <- measure X with binary_measurement (projS S);
+        |   if (hit=1) then Find <- True; else skip;
+        |   call queryG;
+        | }.
+        | program queryH := { on X,Y apply (Uoracle H); }.
+        |
+        | program left := {
+        |  count <- 0;
+        |  (S,G,H,z) <$ o2h_distr;
+        |  call Adv_O2H(Count(queryG));
+        | }.
+        |
+        | program find := {
+        |  count <- 0;
+        |  (S,G,H,z) <$ o2h_distr;
+        |  Find <- False;
+        |  call Adv_O2H(Count(queryGS));
+        | }.
+        |
+        | program right := {
+        |  count <- 0;
+        |  (S,G,H,z) <$ o2h_distr;
+        |  call Adv_O2H(Count(queryH));
+        | }.
+        |
+        | debug:isabelle.
+        |
+        | lemma abs ( Pr[b=1:left(rho)] - Pr[b=1:right(rho)] ) <= 2 * sqrt( (1+real q) * Pr[Find:find(rho)] ).
       """.stripMargin)
 
     val state2 = try {
