isabelle-thys/O2H.thy
@@ -11,24 +11,27 @@ axiomatization binary_measurement :: "('a,'a) bounded \<Rightarrow> (bit,'a) mea
 (* TODO move (& rename?) *)
 definition "projS S = Proj (span {ket s|s. s\<in>S})"
 
-lemma o2h:
+(* TODO remove *)
+definition "PROGRAM_EQUAL x y = (x=y)" for x y :: program
+
+lemma o2h[unfolded PROGRAM_EQUAL_def]:
   fixes q :: nat and b :: "bit variable" and rho :: program_state and count :: "nat variable"
     and Find :: "bool variable" and distr :: "_ distr"
     and z :: "_ variable" and G H :: "('a::universe \<Rightarrow> 'b::{universe,xor_group}) variable" and S :: "'a set variable"
     and adv :: oracle_program and X :: "'a variable" and Y :: "'b variable"
     and in_S :: "bit variable" and Count :: "oracle_program"
 
-  assumes "game_left == block [assign \<lbrakk>count\<rbrakk> Expr[0], sample \<lbrakk>S,G,H,z\<rbrakk> Expr[distr], instantiateOracles adv [instantiateOracles Count [queryG]]]"
-  assumes "game_right == block [assign \<lbrakk>count\<rbrakk> Expr[0], sample \<lbrakk>S,G,H,z\<rbrakk> Expr[distr], instantiateOracles adv [instantiateOracles Count [queryH]]]"
-  assumes "game_find == block [assign \<lbrakk>count\<rbrakk> Expr[0], sample \<lbrakk>S,G,H,z\<rbrakk> Expr[distr], assign \<lbrakk>Find\<rbrakk> Expr[False], instantiateOracles adv [instantiateOracles Count [queryGS]]]"
+  assumes "PROGRAM_EQUAL game_left (block [assign \<lbrakk>count\<rbrakk> Expr[0], sample \<lbrakk>S,G,H,z\<rbrakk> Expr[distr], instantiateOracles adv [instantiateOracles Count [queryG]]])"
+  assumes "PROGRAM_EQUAL game_right (block [assign \<lbrakk>count\<rbrakk> Expr[0], sample \<lbrakk>S,G,H,z\<rbrakk> Expr[distr], instantiateOracles adv [instantiateOracles Count [queryH]]])"
+  assumes "PROGRAM_EQUAL game_find (block [assign \<lbrakk>count\<rbrakk> Expr[0], sample \<lbrakk>S,G,H,z\<rbrakk> Expr[distr], assign \<lbrakk>Find\<rbrakk> Expr[False], instantiateOracles adv [instantiateOracles Count [queryGS]]])"
 
-  assumes "\<forall>P. instantiateOracles Count [P] = block [P, assign \<lbrakk>count\<rbrakk> (expression \<lbrakk>count\<rbrakk> (\<lambda>count. count+1))]"
+  assumes "\<And>P. PROGRAM_EQUAL (instantiateOracles Count [P]) (block [P, assign \<lbrakk>count\<rbrakk> (expression \<lbrakk>count\<rbrakk> (\<lambda>count. count+1))])"
 
-  assumes "queryG = block [qapply \<lbrakk>X,Y\<rbrakk> (expression \<lbrakk>G\<rbrakk> (\<lambda>G. Uoracle G))]"
-  assumes "queryGS = block [measurement \<lbrakk>in_S\<rbrakk> \<lbrakk>X\<rbrakk> (expression \<lbrakk>S\<rbrakk> (\<lambda>S. binary_measurement (projS S))),
+  assumes "PROGRAM_EQUAL queryG (block [qapply \<lbrakk>X,Y\<rbrakk> (expression \<lbrakk>G\<rbrakk> (\<lambda>G. Uoracle G))])"
+  assumes "PROGRAM_EQUAL queryGS (block [measurement \<lbrakk>in_S\<rbrakk> \<lbrakk>X\<rbrakk> (expression \<lbrakk>S\<rbrakk> (\<lambda>S. binary_measurement (projS S))),
                             ifthenelse (expression \<lbrakk>in_S\<rbrakk> (\<lambda>in_S. in_S=1)) [assign \<lbrakk>Find\<rbrakk> Expr[True]] [],
-                            queryG]"
-  assumes "queryH = block [qapply \<lbrakk>X,Y\<rbrakk> (expression \<lbrakk>H\<rbrakk> (\<lambda>H. Uoracle H))]"
+                            queryG])"
+  assumes "PROGRAM_EQUAL queryH (block [qapply \<lbrakk>X,Y\<rbrakk> (expression \<lbrakk>H\<rbrakk> (\<lambda>H. Uoracle H))])"
 
   assumes "distinct_qvars \<lbrakk>b,count,Find,z,G,H,S,in_S,X,Y\<rbrakk>"
 
@@ -44,6 +47,85 @@ lemma o2h:
 
   shows "abs (Pleft - Pright) \<le> 2 * sqrt( (1 + real q)*Pfind )"
     by (cheat O2H)
+
+ML \<open>
+structure O2H = struct
+fun program_body_tac ctxt = SUBGOAL (fn (t,i) =>
+  let val fact = Proof_Context.get_fact ctxt (Facts.named "program_bodies")
+      val progname = case Logic.strip_assums_concl t of
+         Const(\<^const_name>\<open>Trueprop\<close>,_) $ (Const(\<^const_name>\<open>HOL.eq\<close>,_) $ prog $ _) =>
+           Syntax.string_of_term ctxt prog
+       | _ => raise TERM("program_body_tac: internal error",[t])
+  in 
+    Misc.succeed_or_error_tac' (resolve_tac ctxt @{thms trans}) ctxt (K "internal error") i
+  THEN
+    Misc.succeed_or_error_tac' (solve_tac ctxt fact) ctxt (fn _ =>
+           "'" ^ progname ^ "' is not the name of a concrete program") i
+  THEN
+    Misc.succeed_or_error_tac' (resolve_tac ctxt @{thms refl}) ctxt (fn t =>
+          "The body of program '" ^ progname ^ "' is not of the right form for O2H:\n(Problematic equality:" ^
+          Syntax.string_of_term ctxt t ^ ")") i
+  end)
+
+fun free_vars_tac ctxt =
+  let val fact = Proof_Context.get_fact ctxt (Facts.named "program_fv")
+  in SOLVED' (simp_tac (ctxt addsimps fact)) end
+
+fun o2h_tac ctxt = 
+  let val pb_tac = program_body_tac ctxt
+      val fv_tac = free_vars_tac ctxt
+      val resolve_o2h = Misc.succeed_or_error_tac' (resolve_tac ctxt @{thms o2h}) ctxt
+         (K "Goal should be exactly of the form '(Pr[b=1:left(rho)] - Pr[b=1:right(rho)]) <= 2 * sqrt( (1+real q) * Pr[Find:find(rho)])'")
+   in
+    resolve_o2h
+    THEN' pb_tac
+    THEN' pb_tac
+    THEN' pb_tac
+    THEN' pb_tac
+    THEN' pb_tac
+    THEN' pb_tac
+    THEN' pb_tac
+(* TODO: add proper errors *)
+    (* THEN' SOLVED' (simp_tac ctxt) *)
+    (* THEN' fv_tac *)
+  end
+end
+\<close>
+
+named_theorems program_bodies
+named_theorems program_fv
+
+variables classical b :: bit and classical Find :: bool
+  and classical S :: "string set" and classical G :: "string \<Rightarrow> bit" and classical H :: "string \<Rightarrow> bit"
+  and classical z :: "nat list" and classical count :: nat and quantum X :: string and quantum Y :: bit
+and classical in_S :: bit
+begin
+definition test_distr :: "(string set * (string\<Rightarrow>bit) * (string\<Rightarrow>bit) * nat list) distr" where "test_distr = undefined"
+definition adv :: oracle_program where "adv = undefined"
+definition Count :: oracle_program where "Count = undefined"
+
+definition [program_bodies]: "queryG = (block [qapply \<lbrakk>X,Y\<rbrakk> (expression \<lbrakk>var_G\<rbrakk> (\<lambda>G. Uoracle G))])"
+definition [program_bodies]: "queryH = (block [qapply \<lbrakk>X,Y\<rbrakk> (expression \<lbrakk>var_H\<rbrakk> (\<lambda>G. Uoracle G))])"
+definition [program_bodies]: "queryGS =  (block [measurement \<lbrakk>var_in_S\<rbrakk> \<lbrakk>X\<rbrakk> (expression \<lbrakk>var_S\<rbrakk> (\<lambda>S. binary_measurement (projS S))),
+                            ifthenelse (expression \<lbrakk>var_in_S\<rbrakk> (\<lambda>in_S. in_S=1)) [assign \<lbrakk>var_Find\<rbrakk> Expr[True]] [],
+                            queryG])"
+
+definition [program_bodies]: "left = block [assign \<lbrakk>var_count\<rbrakk> (const_expression 0), sample \<lbrakk>var_S, var_G, var_H, var_z\<rbrakk> (const_expression test_distr),
+        instantiateOracles adv [instantiateOracles Count [queryG]]]"
+definition [program_bodies]: "right = block [assign \<lbrakk>var_count\<rbrakk> (const_expression 0), sample \<lbrakk>var_S, var_G, var_H, var_z\<rbrakk> (const_expression test_distr),
+        instantiateOracles adv [instantiateOracles Count [queryH]]]"
+definition [program_bodies]: "findG = (block [assign \<lbrakk>var_count\<rbrakk> Expr[0], sample \<lbrakk>var_S,var_G,var_H,var_z\<rbrakk> Expr[test_distr], assign \<lbrakk>var_Find\<rbrakk> Expr[False], instantiateOracles adv [instantiateOracles Count [queryGS]]])"
+
+lemma [program_bodies]: "instantiateOracles Count [P] = block [P, assign \<lbrakk>c\<rbrakk> (expression \<lbrakk>c\<rbrakk> (\<lambda>count::nat. count + 1))]" for P c 
+  by (cheat Count)
+
+lemma fv_adv[program_fv]: "fv_oracle_program adv = set (variable_names \<lbrakk>X,Y,var_b,var_z\<rbrakk>)" by (cheat fv_adv)
+
+lemma "abs ( Pr[b=1:left(rho)] - Pr[b=1:right(rho)] ) <= 2 * sqrt( (1+real q) * Pr[Find:findG(rho)] )"
+  apply (tactic \<open>O2H.o2h_tac \<^context> 1\<close>)
+  oops
+
+end
 
 end
 
