Empty.thy
@@ -2,4 +2,6 @@ theory Empty
   imports Main
 begin
 
+declare [[show_types,show_consts,show_sorts]]
+
 end
